src/program_proof/tulip/prelude.v
@@ -5,4 +5,4 @@ From Perennial.program_proof.rsm.pure Require Export
   dual_lookup extend fin_maps fin_maps_list fin_sets largest_before list misc nat
   nonexpanding_merge sets vslice word quorum.
 From Perennial.program_proof.tulip Require Export
-  action base cmd encode res msg inv stability.
+  action base cmd encode res msg inv inv_txnlog stability.
