src/program_proof/tulip/program/gcoord/mk_gcoord.v
@@ -1,0 +1,135 @@
+From Perennial.program_proof.tulip.program Require Import prelude.
+From Perennial.program_proof.tulip.program.gcoord Require Import
+  gpreparer_repr greader_repr gcoord_repr.
+  
+Section program.
+  Context `{!heapGS Σ, !tulip_ghostG Σ}.
+
+  Theorem wp_GroupPreparer__reset (gpp : loc) ts gid γ :
+    {{{ own_gpreparer_uninit gpp }}}
+      GroupPreparer__reset #gpp
+    {{{ RET #(); own_gpreparer gpp ts gid γ }}}.
+  Proof.
+    iIntros (Φ) "Hgpp HΦ".
+    wp_rec.
+
+    (*@ func (gpp *GroupPreparer) reset() {                                     @*)
+    (*@     gpp.phase = GPP_VALIDATING                                          @*)
+    (*@     gpp.frespm = make(map[uint64]bool)                                  @*)
+    (*@     gpp.vdm = make(map[uint64]bool)                                     @*)
+    (*@ }                                                                       @*)
+    iNamed "Hgpp".
+    wp_storeField.
+    wp_apply (wp_NewMap u64 bool).
+    iIntros (frespmP') "Hfrespm".
+    wp_storeField.
+    wp_apply (wp_NewMap u64 bool).
+    iIntros (vdmP') "Hvdm".
+    wp_storeField.
+    iApply "HΦ".
+    iFrame "HnrpsP HphaseP HfrespmP HvdmP HsrespmP ∗ %".
+    iExists GPPValidating. simpl.
+    iModIntro.
+    iSplit; first done.
+    iSplit.
+    { iSplit; last done. by iApply big_sepM_empty. }
+    iSplit.
+    { iSplit; last done. by rewrite /validation_responses dom_empty_L big_sepS_empty. }
+    iSplit.
+    { iExists ∅. done. }
+    
+    rewrite Hnrps.
+    simpl.
+    iSplit
+  Admitted.
+
+  Theorem wp_mkGroupPreparer (nrps : u64) gid γ :
+    {{{ True }}}
+      mkGroupPreparer #nrps
+    {{{ (gpp : loc), RET #gpp; own_gpreparer gpp O gid γ }}}.
+  Proof.
+    (*@ func mkGroupPreparer(nrps uint64) *GroupPreparer {                      @*)
+    (*@     gpp := &GroupPreparer{ nrps : nrps }                                @*)
+    (*@     gpp.reset()                                                         @*)
+    (*@                                                                         @*)
+    (*@     return gpp                                                          @*)
+    (*@ }                                                                       @*)
+  Admitted.
+
+  Theorem wp_mkGroupCoordinator (addrmP : loc) (addrm : gmap u64 chan) gid γ :
+    own_map addrmP DfracDiscarded addrm -∗
+    {{{ True }}}
+      mkGroupCoordinator #addrmP
+    {{{ (gcoord : loc), RET #gcoord; is_gcoord gcoord gid γ }}}.
+  Proof.
+    iIntros "#Haddrm" (Φ) "!> _ HΦ".
+    wp_rec.
+
+    (*@ func mkGroupCoordinator(addrm map[uint64]grove_ffi.Address) *GroupCoordinator { @*)
+    (*@     mu := new(sync.Mutex)                                               @*)
+    (*@     cv := sync.NewCond(mu)                                              @*)
+    (*@     cvrs := sync.NewCond(mu)                                            @*)
+    (*@     nrps := uint64(len(addrm))                                          @*)
+    (*@                                                                         @*)
+    wp_apply wp_new_free_lock.
+    iIntros (muP) "Hfree".
+    wp_apply (wp_newCond' with "Hfree").
+    iIntros (cvP) "[Hfree #Hcv]".
+    wp_apply (wp_newCond' with "Hfree").
+    iIntros (cvrsP) "[Hfree #Hcvrs]".
+    wp_apply (wp_MapLen with "Haddrm").
+    iIntros "[%Hnoof _]".
+
+    (*@     var rps = make([]uint64, 0)                                         @*)
+    (*@     for rid := range(addrm) {                                           @*)
+    (*@         rps = append(rps, rid)                                          @*)
+    (*@     }                                                                   @*)
+    (*@                                                                         @*)
+    wp_apply wp_NewSlice.
+    iIntros (rpsP) "Hrps".
+    rewrite uint_nat_W64_0 replicate_0.
+    wp_apply wp_ref_to; first done.
+    iIntros (rpsPP) "HrpsP".
+    set P := (λ (mx : gmap u64 chan), ∃ (rpsP' : Slice.t) (l : list u64),
+                 "HrpsP" ∷ rpsPP ↦[slice.T uint64T] rpsP' ∗
+                 "Hrps"  ∷ own_slice rpsP' uint64T (DfracOwn 1) l ∗
+                 "%Hrps" ∷ ⌜list_to_set l = dom mx⌝)%I.
+    wp_apply (wp_MapIter_fold _ _ _ P with "Haddrm [$Hrps $HrpsP]").
+    { done. }
+    { clear Φ.
+      iIntros (mx rid c Φ) "!> [HP %Hrid] HΦ".
+      iNamed "HP".
+      wp_load.
+      wp_apply (wp_SliceAppend with "Hrps").
+      iIntros (rpsP'') "Hrps".
+      wp_store.
+      iApply "HΦ".
+      iFrame.
+      iPureIntro.
+      rewrite list_to_set_app_L dom_insert_L Hrps /=.
+      set_solver.
+    }
+    iIntros "[_ HP]".
+    iNamed "HP".
+
+    (*@     gcoord := &GroupCoordinator{                                        @*)
+    (*@         rps       : rps,                                                @*)
+    (*@         addrm     : addrm,                                              @*)
+    (*@         mu        : mu,                                                 @*)
+    (*@         cv        : cv,                                                 @*)
+    (*@         cvrs      : cvrs,                                               @*)
+    (*@         idxleader : 0,                                                  @*)
+    (*@         grd       : mkGroupReader(nrps),                                @*)
+    (*@         gpp       : mkGroupPreparer(nrps),                              @*)
+    (*@         tsfinals  : make(map[uint64]bool),                              @*)
+    (*@         conns     : make(map[uint64]grove_ffi.Connection),              @*)
+    (*@     }                                                                   @*)
+    (*@                                                                         @*)
+    wp_load.
+
+    (*@     return gcoord                                                       @*)
+    (*@ }                                                                       @*)
+  Admitted.
+
+
+End program.
